src/ReactorModel/Determinism/InstantaneousStep.lean
@@ -49,6 +49,7 @@ theorem monotonic_progress : (s₁ ⇓ᵢ s₂) → rcn' ∈ s₁.progress → r
 theorem rcn_mem_progress : (e : s₁ ⇓ᵢ s₂) → e.rcn ∈ s₂.progress := 
   (·.mem_progress_iff.mpr $ .inl rfl)
 
+/-
 theorem Skip.equiv : (s₁ ⇓ₛ s₂) → s₁.rtr ≈ s₂.rtr
   | mk .. => .refl
 
@@ -111,6 +112,7 @@ theorem Exec.equiv : (s₁ ⇓ₑ s₂) → s₁.rtr ≈ s₂.rtr
 
 theorem Exec.progress_eq : (e : s₁ ⇓ₑ s₂) → s₂.progress = s₁.progress.insert e.rcn
   | mk .. => rfl
+-/
 
 theorem not_Closed (e : s₁ ⇓ᵢ s₂) : ¬s₁.Closed := by
   intro c
@@ -119,23 +121,18 @@ theorem not_Closed (e : s₁ ⇓ᵢ s₂) : ¬s₁.Closed := by
   sorry -- have := h e.allows.mem.choose
   -- contradiction 
 
-theorem equiv : (s₁ ⇓ᵢ s₂) → s₁.rtr ≈ s₂.rtr
-  | skip e | exec e => e.equiv
+theorem equiv : (s₁ ⇓ᵢ s₂) → s₁.rtr ≈ s₂.rtr :=
+  sorry
 
 theorem deterministic (e₁ : s ⇓ᵢ s₁) (e₂ : s ⇓ᵢ s₂) (h : e₁.rcn = e₂.rcn) : s₁ = s₂ := by
   cases e₁ <;> cases e₂
-  all_goals 
-    case _ e₁ e₂ => 
-      cases e₁; cases e₂
-      simp [rcn] at h
-      subst h
-      first | rfl | contradiction
+  all_goals simp [rcn] at h; subst h; first | rfl | contradiction
 
 theorem acyclic (e : s₁ ⇓ᵢ s₂) : e.rcn ≮[s₁.rtr] e.rcn :=
   e.allows_rcn.acyclic
 
 theorem progress_eq : (e : s₁ ⇓ᵢ s₂) → s₂.progress = s₁.progress.insert e.rcn
-  | skip e | exec e => e.progress_eq  
+  | skip .. | exec .. => rfl
 
 theorem seq_wellordered (e₁ : s₁ ⇓ᵢ s₂) (e₂ : s₂ ⇓ᵢ s₃) : e₂.rcn ≮[s₁.rtr] e₁.rcn := by
   by_contra d
@@ -150,18 +147,16 @@ theorem prepend_indep' (e₁ : s₁ ⇓ᵢ s₂) (e₂ : s₂ ⇓ᵢ s₃) (h : 
       (e₁'.rcn = e₂.rcn) ∧ (e₂'.rcn = e₁.rcn) ∧ (s₃' = s₃) := by
   have hi : _ ≮[_]≯ _ := { not_eq := e₁.seq_rcn_ne e₂, left := h, right := e₁.seq_wellordered e₂ }
   cases e₁ <;> cases e₂ 
-  case skip.skip e₁ e₂ => sorry
-  case skip.exec e₁ e₂ => sorry
-  case exec.skip e₁ e₂ => sorry
-  case exec.exec e₁ e₂ =>
-    
-    cases e₁; cases e₂; case _ rcn₁ ha₁ ht₁ rcn₂ ha₂ ht₂ =>
-      have ha₁' : (s₁.exec rcn₂ |>.record rcn₂).Allows rcn₁ := sorry
-      have ht₁' : (s₁.exec rcn₂ |>.record rcn₂).Triggers rcn₁ := sorry
-      have ha₂' : s₁.Allows rcn₂ := sorry
-      have ht₂' : s₁.Triggers rcn₂ := sorry
-      refine ⟨_, _, Step.exec (Exec.mk ha₂' ht₂'), Step.exec (Exec.mk ha₁' ht₁'), rfl, rfl, ?_⟩
-      
+  case skip.skip => sorry
+  case skip.exec => sorry
+  case exec.skip => sorry
+  case exec.exec rcn₁ ha₁ ht₁ rcn₂ ha₂ ht₂ =>
+    have ha₁' : (s₁.exec rcn₂ |>.record rcn₂).Allows rcn₁ := sorry
+    have ht₁' : (s₁.exec rcn₂ |>.record rcn₂).Triggers rcn₁ := sorry
+    have ha₂' : s₁.Allows rcn₂ := sorry
+    have ht₂' : s₁.Triggers rcn₂ := sorry
+    refine ⟨_, _, Step.exec ha₂' ht₂', Step.exec ha₁' ht₁', rfl, rfl, ?_⟩
+    sorry -- by ext
 
 theorem prepend_indep (e₁ : s₁ ⇓ᵢ s₂) (e₂ : s₂ ⇓ᵢ s₃) (h : e₁.rcn ≮[s₁.rtr] e₂.rcn) :
     ∃ (s₂' : _) (e₁' : s₁ ⇓ᵢ s₂') (e₂' : s₂' ⇓ᵢ s₃), (e₁'.rcn = e₂.rcn) ∧ (e₂'.rcn = e₁.rcn) := by
